---
title: "Multinomial Logit Model"
author: "Yun Kyaw, 251102171"
date: "`r Sys.Date()`"
output: pdf_document
latex_engine: xelatex
---
$$
\begin{aligned}
p_{i1} &= \frac{1}{1+\sum^{J}_{j=2} \exp(\eta_{ij})} \\
p_{ij} &= \frac{\exp(\eta_{ij})}{1+\sum^{J}_{j=2} \exp(\eta_{ij})} \\
\eta_{ij} &= x_i^T\beta_j
\end{aligned}
$$

$$
\begin{aligned}
loglik(\beta_2, ..., \beta_J)
&= \sum_{i=1}^{n} \sum_{j=1}^{J} y_{ij} \log(p_{ij}) + C \\
&= \sum_{i=1}^{n} \left[ y_{i1} \log(p_{i1}) + \sum_{j=2}^{J} y_{ij} \log(p_{ij}) \right]  + C \\
&= \sum_{i=1}^{n} \left[ y_{i1} \log \left(\frac{1}{1+\sum^{J}_{j=2} \exp(\eta_{ij})} \right) + \sum_{j=2}^{J} y_{ij} \log \left(\frac{\exp(\eta_{ij})}{1+\sum^{J}_{j=2} \exp(\eta_{ij})} \right) \right]  + C \\
&= \sum_{i=1}^{n} \left[ y_{i1} \left( \log 1 - \log(1+\sum^{J}_{j=2} \exp(\eta_{ij})) \right) + \sum_{j=2}^{J} y_{ij} \left(\eta_{ij}
- \log(1+\sum^{J}_{j=2} \exp(\eta_{ij}) ) \right) \right]  + C \\
&= \sum_{i=1}^{n} \left[ y_{i1} \left( - \log(1+\sum^{J}_{j=2} \exp(\eta_{ij})) \right) + \sum_{j=2}^{J} y_{ij} \left(\eta_{ij}
- \log(1+\sum^{J}_{j=2} \exp(\eta_{ij}) ) \right) \right]  + C \\
&= \sum_{i=1}^{n} \left[ \sum_{j=2}^{J} y_{ij} \eta_{ij} - y_{i1} \log \left(1+\sum^{J}_{j=2} \exp(\eta_{ij}) \right)
-  \sum_{j=2}^{J} y_{ij} \log \left(1+\sum^{J}_{j=2} \exp(\eta_{ij} ) \right) \right]  + C \\
&= \sum_{i=1}^{n} \left[ \sum_{j=2}^{J} y_{ij} \eta_{ij} - \sum_{j=1}^{J} y_{ij} \log \left(1+\sum^{J}_{j=2} \exp(\eta_{ij} ) \right) \right]  + C \\
&= \sum_{i=1}^{n} \left[ \sum_{j=2}^{J} y_{ij} \eta_{ij} - \log \left(1+\sum^{J}_{j=2} \exp(\eta_{ij})\right) \sum_{j=1}^{J} y_{ij} \right]  + C \\
&= \sum_{i=1}^{n} \left[ \sum_{j=2}^{J} y_{ij} x_i^T\beta_j - \log \left(1+\sum^{J}_{j=2} \exp(x_i^T\beta_j)\right) \sum_{j=1}^{J} y_{ij} \right]  + C \\
\end{aligned}
$$
